Cleaner examples, fast cfold proof using eliminator in DataStruct.v

examples/accumulator.v
@@ -100,7 +100,140 @@ Equations? isPrime (n : nat) : bool :=
     where worker (n' : nat) : bool by rec (k - n') lt :=
     worker i with ge_dec i k :=
       { | left H := true;
-        | right H with eq_nat_dec (Nat.modulo k i) 0 :=
-            { worker i (right H) (left H') := false;
-              worker i (right H) (right H') := worker (S i) } }.
-Proof. clear worker. subst k. do 4 (destruct i; try lia). Defined.
+        | right H := if Nat.eqb (Nat.modulo k i) 0 then false else worker (S i) }.
+Proof. subst k. do 4 (destruct i; try lia). Defined.
+
+Require Import ExtrOcamlBasic.
+
+Extraction isPrime.
+
+(* Definition isPrime_unfold' n := *)
+(*   match n with *)
+(*   | 0 | 1 => false *)
+(*   | 2 | 3 => true *)
+(*   | S (S (S (S k))) => isPrime_unfold_clause_5_worker k 2 *)
+(*   end. *)
+
+(* Lemma isPrime_unfold'_eq n : isPrime n = isPrime_unfold' n. *)
+(* Proof. *)
+(*   revert n. *)
+(*   apply (isPrime_elim (fun n b => b = isPrime_unfold' n) (fun n n' b => b = isPrime_unfold_clause_5_worker n n')); *)
+(*     simpl; try reflexivity. *)
+(*   intros. *)
+(*   unfold isPrime_unfold_clause_5_worker. rewrite Heq. simpl. reflexivity. *)
+(*   intros. *)
+(*   unfold isPrime_unfold_clause_5_worker. rewrite Heq. simpl. *)
+(*   rewrite isPrime_clause_5_worker_unfold_eq. reflexivity. *)
+(* Defined. *)
+
+Equations rev_acc {A} (l : list A) : list A :=
+  rev_acc l := go [] l
+
+   where go : list A -> list A -> list A :=
+         go acc [] := acc;
+         go acc (hd :: tl) := go (hd :: acc) tl.
+
+Lemma rev_acc_eq : forall {A} (l : list A), rev_acc l = rev l.
+Proof.
+  apply (rev_acc_elim (fun A l r => r = rev l)
+                      (fun A _ acc l r => r = rev l ++ acc)); intros; simpl.
+  + now rewrite app_nil_r in H.
+  + reflexivity.
+  + now rewrite H, <- app_assoc.
+Qed.
+
+Equations nat4_discr : nat -> Set :=
+nat4_discr 0 := False;
+nat4_discr 1 := False;
+nat4_discr 2 := False;
+nat4_discr n := True.
+
+Inductive nat4_inv : nat -> Set :=
+| nat4_inv_0 : nat4_inv 0
+| nat4_inv_1 : nat4_inv 1
+| nat4_inv_2 : nat4_inv 2
+| nat4_inv_n n : nat4_discr n -> nat4_inv n.
+
+Equations nat4_view (n : nat) : nat4_inv n :=
+| 0 => nat4_inv_0;
+| 1 => nat4_inv_1;
+| 2 => nat4_inv_2;
+| n => nat4_inv_n n I.
+
+Obligation Tactic := idtac.
+
+Equations? nat4 (n : nat) : nat by rec n lt :=
+nat4 n with nat4_view n :=
+  { nat4 ?(0) nat4_inv_0 := 0;
+    | nat4_inv_1 := 1;
+    | nat4_inv_2 := 1;
+    | nat4_inv_n k Hn := nat4 (pred k) }.
+Proof. destruct k. destruct Hn. auto with arith. Defined.
+
+Inductive three := cone | ctwo | cthree.
+
+Equations discr_three (c : three) : Prop :=
+  discr_three cone := False;
+  discr_three _ := True.
+
+Inductive three_view : three -> Set :=
+| three_one : three_view cone
+| three_other c : discr_three c -> three_view c.
+Equations three_viewc c : three_view c :=
+three_viewc cone := three_one;
+three_viewc c := three_other c I.
+
+Equations onthree (c : three) : three :=
+  onthree c with three_viewc c :=
+  onthree ?(cone) three_one := cone;
+  onthree ?(c) (three_other c Hc) := c.
+Require Import List.
+
+Equations filter_length {A} (l : list A) (f : A -> bool) : length (filter f l) <= length l :=
+ filter_length [] f := le_n 0;
+ filter_length (x :: xs) f with f x :=
+                         { | true => le_n_S _ _ (filter_length xs f);
+                           | false => le_S _ _ (filter_length xs f) }.
+
+Section nubBy.
+  Context {A} (eq : A -> A -> bool).
+
+  Equations? nubBy (l : list A) : list A by rec (length l) lt :=
+  nubBy []        => [];
+  nubBy (x :: xs) => x :: nubBy (filter (fun y => negb (eq x y)) xs).
+  Proof. simpl. auto using filter_length with arith. Defined.
+End nubBy.
+
+Lemma nubBy_length {A} (eq : A -> A -> bool) (l : list A) : length (nubBy eq l) <= length l.
+Proof.
+  funelim (nubBy eq l); simpl; trivial.
+  rewrite (filter_length l) in H. auto with arith.
+Qed.
+
+Lemma In_filter {A} (f : A -> bool) (l : list A) a : In a (filter f l) -> In a l /\ f a = true.
+Proof.
+  induction l; simpl. intros [].
+  destruct (f a0) eqn:Heq.
+  simpl. intuition auto. now subst a0.
+  intuition auto.
+Qed.
+
+Lemma In_nubBy {A} (eq : A -> A -> bool) (l : list A) (a : A) :
+  In a (nubBy eq l) -> In a l.
+Proof.
+  funelim (nubBy eq l).
+  + trivial.
+  + rename a0 into b. intros H0.
+    destruct H0 as [->|H0]; auto. simpl. auto.
+    specialize (H _ H0). apply In_filter in H as [Inal eqa]. right; auto.
+Qed.
+
+Lemma nuBy_nodup {A} (eq : A -> A -> bool) (l : list A) :
+  (forall x y, (eq x y = true) <-> (x = y)) -> NoDup (nubBy eq l).
+Proof.
+  funelim (nubBy eq l). constructor. intros Heq; specialize (H Heq).
+  constructor. intros Hi. apply In_nubBy, In_filter in Hi as [_ eqaa].
+  specialize (Heq a a). destruct (eq a a). discriminate.
+  destruct (proj2 Heq). reflexivity. discriminate.
+  auto.
+Qed.
